dataplane/Examples/Batch/Batch_Op_Tests.thy
@@ -11,18 +11,14 @@ abbreviation "t_1_0 ≡ MyPair (Suc 0) (0 :: nat)"
 abbreviation "t_0_1 ≡ MyPair (0 :: nat) (Suc 0)"
 abbreviation "t_1_1 ≡ MyPair (Suc 0) (Suc 0)"
 
-abbreviation "batch_max ≡ (λ b. if b = [] then trace (STR ''Empty batch! ! !'') [] else [Max (set b)])"
-
-abbreviation "batch_prog inps ≡ compiled_batch_op_opt (λ _. inps) batch_max"
-
 abbreviation "batch_outputs op ≡ lmap (λ io. case io of VOut p (x, t) ⇒ (projr x, t)) (trace_exec op)"
 
 abbreviation "list_inps_test ≡ 
  [Mint t_1_0, Mint t_0_1, Mint t_1_1, Drop t0, Data t_1_1 10, Drop t_1_1, Data t_0_1 7, Data t_1_0 (3 :: nat), Drop t_1_0, Drop t_0_1]"
 abbreviation "inps_test ≡ llist_of list_inps_test"
 
-value [GHC] "unit_test (check_prefix 5500 [((1, 1), (Inr 10, MyPair 1 1)), ((1, 1), (Inr 7, MyPair 0 1)),((1, 1), (Inr 3, MyPair 1 0))] (batch_prog inps_test)) True"
-value [GHC] "unit_test (batch_outputs (batch_prog inps_test)) (llist_of [(7, MyPair 0 1), (10, MyPair 1 1), (3, MyPair 1 0)])"
+value [GHC] "unit_test (check_prefix 5500 [((1, 1), (Inr 10, MyPair 1 1)), ((1, 1), (Inr 7, MyPair 0 1)),((1, 1), (Inr 3, MyPair 1 0))] (compile_dataflow_opt (λ _. []) (batch_tree (λ _. inps_test) batch_max))) True"
+value [GHC] "unit_test (batch_outputs (compile_dataflow_opt (λ _. []) (batch_tree (λ _. inps_test) batch_max))) (llist_of [(7, MyPair 0 1), (10, MyPair 1 1), (3, MyPair 1 0)])"
 
 abbreviation "list_inps_test2 ≡ 
  [ Mint t_1_0, Data t_1_0 10, Data t0 (7 :: nat), Drop t0, Drop t_1_0]"
@@ -35,25 +31,22 @@ text ‹Pruning the nops keeps the choice tree finite, so the search below
   @{thm [source] dataflow_opt_op_wbisim_start}, whose @{term nop_invar}
   hypothesis is discharged in theory Batch_op_Nop_Invariant.›
 
-value [GHC] "unit_test (check_prefix 55500 [((1, 1), (Inr 7, MyPair 0 0))] (batch_prog inps_test2)) True"
-value [GHC] "unit_test (check_prefix 55500 [((1, 1), (Inr 10, MyPair 1 0))] (batch_prog inps_test2)) True"
+value [GHC] "unit_test (check_prefix 55500 [((1, 1), (Inr 7, MyPair 0 0))] (compile_dataflow_opt (λ _. []) (batch_tree (λ _. inps_test2) batch_max))) True"
+value [GHC] "unit_test (check_prefix 55500 [((1, 1), (Inr 10, MyPair 1 0))] (compile_dataflow_opt (λ _. []) (batch_tree (λ _. inps_test2) batch_max))) True"
 
-value [GHC] "unit_test (check_prefix 55500 [((1, 1), (Inr 7, MyPair 0 0)), ((1, 1), (Inr 10, MyPair 1 0))] (batch_prog inps_test2)) True"
-value [GHC] "unit_test (check_prefix 55500 [((1, 1), (Inr 10, MyPair 1 0)), ((1, 1), (Inr 7, MyPair 0 0))] (batch_prog inps_test2)) True"
+value [GHC] "unit_test (check_prefix 55500 [((1, 1), (Inr 7, MyPair 0 0)), ((1, 1), (Inr 10, MyPair 1 0))] (compile_dataflow_opt (λ _. []) (batch_tree (λ _. inps_test2) batch_max))) True"
+value [GHC] "unit_test (check_prefix 55500 [((1, 1), (Inr 10, MyPair 1 0)), ((1, 1), (Inr 7, MyPair 0 0))] (compile_dataflow_opt (λ _. []) (batch_tree (λ _. inps_test2) batch_max))) True"
 
-value [GHC] "unit_test (check_prefix 5500 [((1, 1), (Inr 7, MyPair 0 1)), ((1, 1), (Inr 10, MyPair 1 1)), ((1, 1), (Inr 3, MyPair 1 0))] (batch_prog inps_test)) True"
+value [GHC] "unit_test (check_prefix 5500 [((1, 1), (Inr 7, MyPair 0 1)), ((1, 1), (Inr 10, MyPair 1 1)), ((1, 1), (Inr 3, MyPair 1 0))] (compile_dataflow_opt (λ _. []) (batch_tree (λ _. inps_test) batch_max))) True"
 
 section ‹Trace-Nondeterminism on Two Incomparable Timestamps›
 
-text ‹The stream below is the one drawn in the thesis figure.›
-
-abbreviation "list_inps_test3 ≡
- [Mint t_1_0, Mint t_0_1, Drop t0, Data t_1_0 (10 :: nat), Data t_0_1 7,
-  Drop t_0_1, Drop t_1_0]"
-abbreviation "inps_test3 ≡ llist_of list_inps_test3"
+text ‹The stream ‹inps› and the program ‹prog› below are defined at the
+  end of theory ‹Batch_Op›, and they are the ones drawn in the thesis
+  figure.›
 
 text ‹Frontier-driven order.›
-value [GHC] "unit_test (check_prefix 55500 [((1, 1), (Inr 7, MyPair 0 1)), ((1, 1), (Inr 10, MyPair 1 0))] (batch_prog inps_test3)) True"
+value [GHC] "unit_test (check_prefix 55500 [((1, 1), (Inr 7, MyPair 0 1)), ((1, 1), (Inr 10, MyPair 1 0))] prog) True"
 (* WARNING: the check above takes about twelve minutes. The schedule it looks
    for pauses the input operator between its two drops, and the depth-first
    search of check_prefix only reaches it after exploring every schedule that
@@ -62,16 +55,16 @@ value [GHC] "unit_test (check_prefix 55500 [((1, 1), (Inr 7, MyPair 0 1)), ((1, 
 
 text ‹Consumption-driven order.›
 
-value [GHC] "unit_test (check_prefix 55500 [((1, 1), (Inr 10, MyPair 1 0)), ((1, 1), (Inr 7, MyPair 0 1))] (batch_prog inps_test3)) True"
+value [GHC] "unit_test (check_prefix 55500 [((1, 1), (Inr 10, MyPair 1 0)), ((1, 1), (Inr 7, MyPair 0 1))] prog) True"
 
 (* No schedule pairs the batch of t_1_0 with the timestamp t_0_1. Answering
    that negatively means ruling out every schedule, which explores the whole
    choice tree, so this check is left disabled. 
-value [GHC] "unit_test (check_prefix 55500 [((1, 1), (Inr 10, MyPair 0 1))] (batch_prog inps_test3)) False"
+value [GHC] "unit_test (check_prefix 55500 [((1, 1), (Inr 10, MyPair 0 1))] prog) False"
  *)
 
 text ‹The single schedule of @{const trace_exec}, without any search.›
 
-value [GHC] "unit_test (batch_outputs (batch_prog inps_test3)) (llist_of [(10, MyPair 1 0), (7, MyPair 0 1)])"
+value [GHC] "unit_test (batch_outputs prog) (llist_of [(10, MyPair 1 0), (7, MyPair 0 1)])"
 
 end
